---
title: "Formulae"
author: "Econometrics"
institute: "Nova School of Business and Economics"
format: html
---

::: {.columns}

::: {.column}
* $Y_i = \beta_0 + \beta_1 x_1^i + \dots + \beta_k X^k_i + u_i$

* $\hat{\beta}_j = \frac{\sum_{i=1}^n (x_i^j - \bar{x}^j)(y_i - \bar{y})}{\sum_{i=1}^n (x_i^j - \bar{x}^j)^2}$

* $\hat{\beta}_0 = \bar{y}-\sum_j \beta_j\bar{x}^j$

:::

::: {.column}

* $Y = X\beta + u$

* $\hat{\beta} = \left(X'X\right)^{-1}X'y$

* $V\left[\hat{\beta}\right]=\sigma^2 \left(X'X\right)^{-1}$

:::

:::

* $R^2 = 1 - \frac{\sum_{i=1}^n (Y_i - \hat{Y}_i)^2}{\sum_{i=1}^n (Y_i - \bar{Y})^2}$
 
$$SST=SSE+SSR$$
 
$$\hat{\sigma}^2 = \frac{SSR}{n-2}$$
 
$$SE(\hat{\beta}_1) = \sqrt{\frac{\hat{\sigma}^2}{\sum_{i=1}^n (X_i - \bar{X})^2}}$$
 
$$Y_i = \beta_0 + \beta_1 X_{i1} + \dots + \beta_k X_{ik} + u_i$$
 
$$Y = X \beta + u$$
 
$$\hat{\beta} = (X' X)^{-1} X' Y$$
 
$$\widehat{Var}(\hat{\beta}) = \hat{\sigma}^2 (X' X)^{-1}$$
 
$$\bar{R}^2 = 1 - (1 - R^2) \frac{n-1}{n-k-1}$$
 
$$t = \frac{\hat{\beta}_j - c}{SE(\hat{\beta}_j)}$$
 
$$\hat{\beta}_j \pm t_{\alpha/2, n-k-1} \cdot SE(\hat{\beta}_j)$$
 
$$F = \frac{R^2/k}{(1-R^2)/(n-k-1)}\sim F_{(k,n-k-1)}$$
 
$$F = \frac{(SSR_r - SSR_{ur})/q}{SSR_{ur}/(n-k-1)}=\frac{(R^2_{ur}-R^2_r)/q}{(1-R^2_{ur})/(n-k-1)}$$
 
$$\widehat{\text{Var}}_{\text{HR}}(\hat{\beta}) = (X' X)^{-1} \left( \sum_{i=1}^n \hat{u}_i^2 X_i X_i' \right) (X' X)^{-1}$$